veric/invariants.v
@@ -1,0 +1,143 @@
+Set Warnings "-notation-overridden,-custom-entry-overridden,-hiding-delimiting-key".
+From VST.veric Require Import res_predicates mpred lifting_expr lifting.
+Set Warnings "notation-overridden,custom-entry-overridden,hiding-delimiting-key".
+
+Section VST.
+
+Context `{!VSTGS OK_ty Σ}.
+
+  Definition inv `{!VSTGS OK_ty Σ} N (P : assert) := ∃ n, stack_level n ∗ ⎡inv N (P n)⎤.
+
+  Global Instance inv_contractive N : Contractive (inv N).
+  Proof. solve_contractive. Qed.
+
+  Global Instance inv_ne N : NonExpansive (inv N).
+  Proof. apply contractive_ne, _. Qed.
+
+  Global Instance inv_proper N : Proper (equiv ==> equiv) (inv N).
+  Proof. apply ne_proper, _. Qed.
+
+  Global Instance inv_persistent N P : Persistent (inv N P).
+  Proof. apply _. Qed.
+
+  Global Instance inv_affine N P : Affine (inv N P).
+  Proof. apply _. Qed.
+
+  Lemma inv_alter N P Q : ⊢ inv N P -∗ □ ▷ (P -∗ Q ∗ (Q -∗ P)) -∗ inv N Q.
+  Proof.
+    split => n; rewrite /inv /stack_level; monPred.unseal.
+    iIntros "_" (? ->) "(% & L & HI) % -> #HPQ".
+    rewrite monPred_at_affinely monPred_at_intuitionistically /=; iDestruct "L" as %->.
+    iExists _; rewrite monPred_at_affinely; iSplit => //.
+    iApply (inv_alter with "HI").
+    iIntros "!> !> HP".
+    iDestruct ("HPQ" with "[//] HP") as "($ & HQ)".
+    by iApply "HQ".
+  Qed.
+
+  Lemma inv_iff N P Q : ⊢ inv N P -∗ □ ▷ (P ∗-∗ Q) -∗ inv N Q.
+  Proof.
+    iIntros "#HI #HPQ". iApply (inv_alter with "HI").
+    iIntros "!> !> HP". iSplitL "HP".
+    - by iApply "HPQ".
+    - iIntros "HQ". by iApply "HPQ".
+  Qed.
+
+  Lemma inv_alloc N E P : ▷ P ⊢ |={E}=> inv N P.
+  Proof.
+    split => n; rewrite /inv /stack_level; monPred.unseal.
+    iIntros "HP".
+    iMod (inv_alloc with "HP") as "$".
+    rewrite monPred_at_affinely //.
+  Qed.
+
+  Lemma inv_alloc_open N E P :
+    ↑N ⊆ E → ⊢ |={E, E∖↑N}=> inv N P ∗ (▷P ={E∖↑N, E}=∗ emp).
+  Proof.
+    split => n; rewrite /inv /stack_level; monPred.unseal.
+    iIntros "_". iMod inv_alloc_open as "[$ Hclose]"; first done.
+    iModIntro.
+    rewrite monPred_at_affinely; iSplit => //.
+    by iIntros (? ->).
+  Qed.
+
+  Lemma inv_acc E N P :
+    ↑N ⊆ E → inv N P ⊢ |={E,E∖↑N}=> ▷ P ∗ (▷ P ={E∖↑N,E}=∗ emp).
+  Proof.
+    split => n; rewrite /inv /stack_level; monPred.unseal.
+    iIntros "(% & L & HI)".
+    rewrite monPred_at_affinely; iDestruct "L" as %->.
+    iMod (inv_acc with "HI") as "($ & HI)"; first done.
+    by iIntros "!>" (? ->).
+  Qed.
+
+  Lemma inv_combine N1 N2 N P Q :
+    N1 ## N2 →
+    ↑N1 ∪ ↑N2 ⊆@{coPset} ↑N →
+    ⊢ inv N1 P -∗ inv N2 Q -∗ inv N (P ∗ Q).
+  Proof.
+    split => n; rewrite /inv /stack_level; monPred.unseal.
+    iIntros "_" (? ->) "(% & L1 & HI1) % -> (% & L2 & HI2)".
+    iDestruct (inv_combine with "HI1 HI2") as "HI"; [done..|].
+    iExists j0; rewrite !monPred_at_affinely; iDestruct "L1" as %->; iDestruct "L2" as %->.
+    by iFrame.
+  Qed.
+
+(*  Lemma except_0_inv N P : ◇ inv N P ⊢ inv N P.
+  Proof.
+    rewrite inv_unseal /inv_def. Search bi_except_0 Affine.
+  Qed.*)
+
+  (** ** Proof mode integration *)
+(*  Global Instance is_except_0_inv N P : IsExcept0 (inv N P).
+  Proof. apply except_0_inv. Qed.*)
+
+  Global Instance into_inv_inv N P : IntoInv (inv N P) N := {}.
+
+  Global Instance into_acc_inv N P E:
+    IntoAcc (X := unit) (inv N P)
+            (↑N ⊆ E) emp (fupd E (E ∖ ↑N)) (fupd (E ∖ ↑N) E)
+            (λ _ : (), (▷ P)%I) (λ _ : (), (▷ P)%I) (λ _ : (), None).
+  Proof.
+    rewrite /IntoAcc /accessor bi.exist_unit.
+    iIntros (?) "#Hinv _". by iApply inv_acc.
+  Qed.
+
+  (** ** Derived properties *)
+  Lemma inv_acc_strong E N P :
+    ↑N ⊆ E → inv N P ⊢ |={E,E∖↑N}=> ▷ P ∗ ∀ E', ▷ P ={E',↑N ∪ E'}=∗ emp.
+  Proof.
+    iIntros (?) "Hinv".
+    iPoseProof (inv_acc (↑ N) N with "Hinv") as "H"; first done.
+    rewrite difference_diag_L.
+    iPoseProof (fupd_mask_frame_r _ _ (E ∖ ↑ N) with "H") as "H"; first set_solver.
+    rewrite left_id_L -union_difference_L //. iMod "H" as "[$ H]"; iModIntro.
+    iIntros (E') "HP".
+    iPoseProof (fupd_mask_frame_r _ _ E' with "(H HP)") as "H"; first set_solver.
+    by rewrite left_id_L.
+  Qed.
+
+  Lemma inv_acc_timeless E N P `{!Timeless P} :
+    ↑N ⊆ E → inv N P ⊢ |={E,E∖↑N}=> P ∗ (P ={E∖↑N,E}=∗ emp).
+  Proof.
+    iIntros (?) "Hinv". iMod (inv_acc with "Hinv") as "[>HP Hclose]"; auto.
+    iIntros "!> {$HP} HP". iApply "Hclose"; auto.
+  Qed.
+
+  Lemma inv_split_l N P Q : inv N (P ∗ Q) ⊢ inv N P.
+  Proof.
+    iIntros "#HI". iApply inv_alter; eauto.
+    iIntros "!> !> [$ $] $".
+  Qed.
+  Lemma inv_split_r N P Q : inv N (P ∗ Q) ⊢ inv N Q.
+  Proof.
+    rewrite (comm _ P Q). eapply inv_split_l.
+  Qed.
+  Lemma inv_split N P Q : inv N (P ∗ Q) ⊢ inv N P ∗ inv N Q.
+  Proof.
+    iIntros "#H".
+    iPoseProof (inv_split_l with "H") as "$".
+    iPoseProof (inv_split_r with "H") as "$".
+  Qed.
+
+End VST.
